tests/TestsBuiltin_ExeCtrl.thy
@@ -31,20 +31,20 @@ begin
       }
 *)
 (*
-value "multi_step tre0_ex1 (gstk_C1 # []) 1 100"
-value "multi_step tre0_ex1 (gstk_C1 # []) 2 100"
-value "multi_step tre0_ex1 (gstk_C1 # []) 3 100"
-value "multi_step tre0_ex1 (gstk_C1 # []) 4 100"
-value "multi_step tre0_ex1 (gstk_C1 # []) 5 100"
-value "multi_step tre0_ex1 (gstk_C1 # []) 6 100"
-value "multi_step tre0_ex1 (gstk_C1 # []) 7 100"
+value "multi_step tre0_ex1 (gstk_C1 # []) 1"
+value "multi_step tre0_ex1 (gstk_C1 # []) 2"
+value "multi_step tre0_ex1 (gstk_C1 # []) 3"
+value "multi_step tre0_ex1 (gstk_C1 # []) 4"
+value "multi_step tre0_ex1 (gstk_C1 # []) 5"
+value "multi_step tre0_ex1 (gstk_C1 # []) 6"
+value "multi_step tre0_ex1 (gstk_C1 # []) 7"
 *)
 
-value "check_var_val_stp (multi_step tre0_ex1 (gstk_C1 # []) 6 100) [(- 122, (NL 1) :L U256)]" 
+value "check_var_val_stp (multi_step tre0_ex1 (gstk_C1 # []) 6) [(- 122, (NL 1) :L U256)]" 
 
-value "check_gs_gas_stp (multi_step tre0_ex1 (gstk_C1 # []) 5 100) (3000000-705)"
+value "check_gs_gas_stp (multi_step tre0_ex1 (gstk_C1 # []) 5) (3000000-705)"
 
-value "\<not> check_gstk_exc_stp (multi_step tre0_ex1 (gstk_C1 # []) 7 100)"
+value "\<not> check_gstk_exc_stp (multi_step tre0_ex1 (gstk_C1 # []) 7)"
 
 
 (*C2 --- (a=0,xx=0) \<rightarrow>* (a=0,xx=99)
@@ -57,20 +57,20 @@ value "\<not> check_gstk_exc_stp (multi_step tre0_ex1 (gstk_C1 # []) 7 100)"
 *)
 (*call \<rightarrow>* exception, due to insufficient balance *)
 (*
-value "multi_step tre0_ex1 gstk_C2 1 10"
-value "multi_step tre0_ex1 gstk_C2 2 10"
-value "multi_step tre0_ex1 gstk_C2 3 10"
-value "multi_step tre0_ex1 gstk_C2 4 10"
-value "multi_step tre0_ex1 gstk_C2 5 10"
-value "multi_step tre0_ex1 gstk_C2 6 10"
+value "multi_step tre0_ex1 gstk_C2 1"
+value "multi_step tre0_ex1 gstk_C2 2"
+value "multi_step tre0_ex1 gstk_C2 3"
+value "multi_step tre0_ex1 gstk_C2 4"
+value "multi_step tre0_ex1 gstk_C2 5"
+value "multi_step tre0_ex1 gstk_C2 6"
 *)
 
-value "check_var_val_stp (multi_step tre0_ex1 gstk_C2 5 10)
+value "check_var_val_stp (multi_step tre0_ex1 gstk_C2 5)
   [(xx_id, (NL 99) :L U256),(a_id, (NL 0) :L U256)]" 
 
-value "check_gs_gas_stp (multi_step tre0_ex1 gstk_C2 6 10) (3000000-14)"
+value "check_gs_gas_stp (multi_step tre0_ex1 gstk_C2 6) (3000000-14)"
 
-value "check_gstk_exc_stp (multi_step tre0_ex1 gstk_C2 2 10)"
+value "check_gstk_exc_stp (multi_step tre0_ex1 gstk_C2 2)"
 
 
 (*C3 ---(xx=28,y=0) \<rightarrow>* (xx=1,y=400)
@@ -81,21 +81,21 @@ value "check_gstk_exc_stp (multi_step tre0_ex1 gstk_C2 2 10)"
      callee{ }
 *)
 (*
-value "multi_step tre0_ex1 gstk_C3 1 10"
-value "multi_step tre0_ex1 gstk_C3 2 10"
-value "multi_step tre0_ex1 gstk_C3 3 10"
-value "multi_step tre0_ex1 gstk_C3 4 10"
-value "multi_step tre0_ex1 gstk_C3 5 10"
-value "multi_step tre0_ex1 gstk_C3 6 10"
-value "multi_step tre0_ex1 gstk_C3 7 10"
+value "multi_step tre0_ex1 gstk_C3 1"
+value "multi_step tre0_ex1 gstk_C3 2"
+value "multi_step tre0_ex1 gstk_C3 3"
+value "multi_step tre0_ex1 gstk_C3 4"
+value "multi_step tre0_ex1 gstk_C3 5"
+value "multi_step tre0_ex1 gstk_C3 6"
+value "multi_step tre0_ex1 gstk_C3 7"
 *)
 
-value "check_var_val_stp (multi_step tre0_ex1 gstk_C3 6 10)
+value "check_var_val_stp (multi_step tre0_ex1 gstk_C3 6)
   [(xx_id, (NL 1) :L U256),(y_id, (NL 400) :L U256)]" 
 
-value "check_gs_gas_stp (multi_step tre0_ex1 gstk_C3 4 10) (3000000-9700)"
+value "check_gs_gas_stp (multi_step tre0_ex1 gstk_C3 4) (3000000-9700)"
 
-value "\<not> check_gstk_exc_stp (multi_step tre0_ex1 gstk_C3 4 10)"
+value "\<not> check_gstk_exc_stp (multi_step tre0_ex1 gstk_C3 4)"
 
 
 (*C4 --- (xx=28,y=0) \<rightarrow>* (xx=1,y=400)
@@ -106,21 +106,21 @@ value "\<not> check_gstk_exc_stp (multi_step tre0_ex1 gstk_C3 4 10)"
     callcodeblk{ }
 *)
 (*
-value "multi_step tre0_ex1 gstk_C4 1 10"
-value "multi_step tre0_ex1 gstk_C4 2 10"
-value "multi_step tre0_ex1 gstk_C4 3 10"
-value "multi_step tre0_ex1 gstk_C4 4 10"
-value "multi_step tre0_ex1 gstk_C4 5 10"
-value "multi_step tre0_ex1 gstk_C4 6 10"
-value "multi_step tre0_ex1 gstk_C4 7 10"
+value "multi_step tre0_ex1 gstk_C4 1"
+value "multi_step tre0_ex1 gstk_C4 2"
+value "multi_step tre0_ex1 gstk_C4 3"
+value "multi_step tre0_ex1 gstk_C4 4"
+value "multi_step tre0_ex1 gstk_C4 5"
+value "multi_step tre0_ex1 gstk_C4 6"
+value "multi_step tre0_ex1 gstk_C4 7"
 *)
 
-value "check_var_val_stp (multi_step tre0_ex1 gstk_C4 6 10)
+value "check_var_val_stp (multi_step tre0_ex1 gstk_C4 6)
   [(xx_id, (NL 1) :L U256),(y_id, (NL 400) :L U256)]" 
 
-value "check_gs_gas_stp (multi_step tre0_ex1 gstk_C4 4 10) (3000000-9700)"
+value "check_gs_gas_stp (multi_step tre0_ex1 gstk_C4 4) (3000000-9700)"
 
-value "\<not> check_gstk_exc_stp (multi_step tre0_ex1 gstk_C4 4 10)"
+value "\<not> check_gstk_exc_stp (multi_step tre0_ex1 gstk_C4 4)"
 
 
 (*C5 ---(xx=28,y=0) \<rightarrow>* (xx=1,y=400)
@@ -131,21 +131,21 @@ value "\<not> check_gstk_exc_stp (multi_step tre0_ex1 gstk_C4 4 10)"
     delcallblk{ }
 *)
 (*
-value "multi_step tre0_ex1 gstk_C5 1 10"
-value "multi_step tre0_ex1 gstk_C5 2 10"
-value "multi_step tre0_ex1 gstk_C5 3 10"
-value "multi_step tre0_ex1 gstk_C5 4 10"
-value "multi_step tre0_ex1 gstk_C5 5 10"
-value "multi_step tre0_ex1 gstk_C5 6 10"
-value "multi_step tre0_ex1 gstk_C5 7 10"
+value "multi_step tre0_ex1 gstk_C5 1"
+value "multi_step tre0_ex1 gstk_C5 2"
+value "multi_step tre0_ex1 gstk_C5 3"
+value "multi_step tre0_ex1 gstk_C5 4"
+value "multi_step tre0_ex1 gstk_C5 5"
+value "multi_step tre0_ex1 gstk_C5 6"
+value "multi_step tre0_ex1 gstk_C5 7"
 *)
 
-value "check_var_val_stp (multi_step tre0_ex1 gstk_C5 6 10)
+value "check_var_val_stp (multi_step tre0_ex1 gstk_C5 6)
   [(xx_id, (NL 1) :L U256),(y_id, (NL 400) :L U256)]" 
 
-value "check_gs_gas_stp (multi_step tre0_ex1 gstk_C5 4 10) (3000000-700)"
+value "check_gs_gas_stp (multi_step tre0_ex1 gstk_C5 4) (3000000-700)"
 
-value "\<not> check_gstk_exc_stp (multi_step tre0_ex1 gstk_C5 4 10)"
+value "\<not> check_gstk_exc_stp (multi_step tre0_ex1 gstk_C5 4)"
 
 
 (*C6 ---
@@ -159,18 +159,18 @@ value "\<not> check_gstk_exc_stp (multi_step tre0_ex1 gstk_C5 4 10)"
           }
 *)
 (*
-value "multi_step tre0_ex1 gstk_C6 1 10"
-value "multi_step tre0_ex1 gstk_C6 2 10"
-value "multi_step tre0_ex1 gstk_C6 3 10"
-value "multi_step tre0_ex1 gstk_C6 4 10"
-value "multi_step tre0_ex1 gstk_C6 5 10"
-value "multi_step tre0_ex1 gstk_C6 6 10"
-value "multi_step tre0_ex1 gstk_C6 7 10"
+value "multi_step tre0_ex1 gstk_C6 1"
+value "multi_step tre0_ex1 gstk_C6 2"
+value "multi_step tre0_ex1 gstk_C6 3"
+value "multi_step tre0_ex1 gstk_C6 4"
+value "multi_step tre0_ex1 gstk_C6 5"
+value "multi_step tre0_ex1 gstk_C6 6"
+value "multi_step tre0_ex1 gstk_C6 7"
 *)
 
-value "check_var_val_stp (multi_step tre0_ex1 gstk_C6 6 10) [(h_id, TL :L Bool)]" 
+value "check_var_val_stp (multi_step tre0_ex1 gstk_C6 6) [(h_id, TL :L Bool)]" 
 
-value "\<not> check_gstk_exc_stp (multi_step tre0_ex1 gstk_C6 6 10)"
+value "\<not> check_gstk_exc_stp (multi_step tre0_ex1 gstk_C6 6)"
 
 
 (*C7 ---
@@ -184,32 +184,32 @@ value "\<not> check_gstk_exc_stp (multi_step tre0_ex1 gstk_C6 6 10)"
           }
 *)
 (*
-value "multi_step tre0_ex1 gstk_C7 1 10"
-value "multi_step tre0_ex1 gstk_C7 2 10"
-value "multi_step tre0_ex1 gstk_C7 3 10"
-value "multi_step tre0_ex1 gstk_C7 4 10"
-value "multi_step tre0_ex1 gstk_C7 5 10"
-value "multi_step tre0_ex1 gstk_C7 6 10"
+value "multi_step tre0_ex1 gstk_C7 1"
+value "multi_step tre0_ex1 gstk_C7 2"
+value "multi_step tre0_ex1 gstk_C7 3"
+value "multi_step tre0_ex1 gstk_C7 4"
+value "multi_step tre0_ex1 gstk_C7 5"
+value "multi_step tre0_ex1 gstk_C7 6"
 *)
 
-value "check_var_val_stp (multi_step tre0_ex1 gstk_C7 5 10) [(h_id, TL :L Bool)]" 
+value "check_var_val_stp (multi_step tre0_ex1 gstk_C7 5) [(h_id, TL :L Bool)]" 
 
-value "check_gs_gas_stp (multi_step tre0_ex1 gstk_C7 3 10) (3000000-3-0)"
+value "check_gs_gas_stp (multi_step tre0_ex1 gstk_C7 3) (3000000-3-0)"
 
-value "\<not> check_gstk_exc_stp (multi_step tre0_ex1 gstk_C7 6 10)"
+value "\<not> check_gstk_exc_stp (multi_step tre0_ex1 gstk_C7 6)"
 
 
 (*C8 ---
    selfdestruct(1)
 *)
 (*
-value "multi_step tre0_ex1 gstk_C8 1 20"  
-value "multi_step tre0_ex1 gstk_C8 2 20"  
+value "multi_step tre0_ex1 gstk_C8 1"  
+value "multi_step tre0_ex1 gstk_C8 2"  
 *)
 
-value "check_gs_gas_stp (multi_step tre0_ex1 gstk_C8 2 20) (3000000-5000)"
+value "check_gs_gas_stp (multi_step tre0_ex1 gstk_C8 2) (3000000-5000)"
 
-value "\<not> check_gstk_exc_stp (multi_step tre0_ex1 gstk_C8 2 20)"
+value "\<not> check_gstk_exc_stp (multi_step tre0_ex1 gstk_C8 2)"
 
 
 (*C9 ---
@@ -217,94 +217,94 @@ value "\<not> check_gstk_exc_stp (multi_step tre0_ex1 gstk_C8 2 20)"
 *)
 
 (*
-value "multi_step tre0_ex1 gstk_C9 1 20"
-value "multi_step tre0_ex1 gstk_C9 2 20"
-value "multi_step tre0_ex1 gstk_C9 3 20"
+value "multi_step tre0_ex1 gstk_C9 1"
+value "multi_step tre0_ex1 gstk_C9 2"
+value "multi_step tre0_ex1 gstk_C9 3"
 *)
 
-value "check_gs_gas_stp (multi_step tre0_ex1 gstk_C9 2 20) (3000000-(375+8*32+0))"
+value "check_gs_gas_stp (multi_step tre0_ex1 gstk_C9 2) (3000000-(375+8*32+0))"
 
-value "\<not> check_gstk_exc_stp (multi_step tre0_ex1 gstk_C9 3 20)"
+value "\<not> check_gstk_exc_stp (multi_step tre0_ex1 gstk_C9 3)"
 
 
 (*C10 ---
    log1(0x1,0x20,0x24 )
 *)
 (*
-value "multi_step tre0_ex1 gstk_C10 1 20"
-value "multi_step tre0_ex1 gstk_C10 2 20"
-value "multi_step tre0_ex1 gstk_C10 3 20"
+value "multi_step tre0_ex1 gstk_C10 1"
+value "multi_step tre0_ex1 gstk_C10 2"
+value "multi_step tre0_ex1 gstk_C10 3"
 *)
 
-value "check_gs_gas_stp (multi_step tre0_ex1 gstk_C10 2 20) (3000000-(375+8*32+375))"
+value "check_gs_gas_stp (multi_step tre0_ex1 gstk_C10 2) (3000000-(375+8*32+375))"
 
-value "\<not> check_gstk_exc_stp (multi_step tre0_ex1 gstk_C10 3 20)"
+value "\<not> check_gstk_exc_stp (multi_step tre0_ex1 gstk_C10 3)"
 
 
 (*C11 ---
   log2(0x1,0x20,0x24,0x31)
 *)
 (*
-value "multi_step tre0_ex1 gstk_C11 1 20"
-value "multi_step tre0_ex1 gstk_C11 2 20"
-value "multi_step tre0_ex1 gstk_C11 3 20"
+value "multi_step tre0_ex1 gstk_C11 1"
+value "multi_step tre0_ex1 gstk_C11 2"
+value "multi_step tre0_ex1 gstk_C11 3"
 *)
 
-value "check_gs_gas_stp (multi_step tre0_ex1 gstk_C11 2 20) (3000000-(375+8*32+375*2))"
+value "check_gs_gas_stp (multi_step tre0_ex1 gstk_C11 2) (3000000-(375+8*32+375*2))"
 
-value "\<not> check_gstk_exc_stp (multi_step tre0_ex1 gstk_C11 3 20)"
+value "\<not> check_gstk_exc_stp (multi_step tre0_ex1 gstk_C11 3)"
 
 
 (*C12 ---
   log3(0x1,0x20,0x24,0x31,0x3a)
 *)
 (*
-value "multi_step tre0_ex1 gstk_C12 1 20"
-value "multi_step tre0_ex1 gstk_C12 2 20"
-value "multi_step tre0_ex1 gstk_C12 3 20"
+value "multi_step tre0_ex1 gstk_C12 1"
+value "multi_step tre0_ex1 gstk_C12 2"
+value "multi_step tre0_ex1 gstk_C12 3"
 *)
 
-value "check_gs_gas_stp (multi_step tre0_ex1 gstk_C12 2 20) (3000000-(375+8*32+375*3))"
+value "check_gs_gas_stp (multi_step tre0_ex1 gstk_C12 2) (3000000-(375+8*32+375*3))"
 
-value "\<not> check_gstk_exc_stp (multi_step tre0_ex1 gstk_C12 3 20)"
+value "\<not> check_gstk_exc_stp (multi_step tre0_ex1 gstk_C12 3)"
 
 
 (*C13 ---
   log4(0x1,0x20,0x24,0x31,0x3a,0x44)
 *)
 (*
-value "multi_step tre0_ex1 gstk_C13 1 20"
-value "multi_step tre0_ex1 gstk_C13 2 20"
-value "multi_step tre0_ex1 gstk_C13 3 20"
+value "multi_step tre0_ex1 gstk_C13 1"
+value "multi_step tre0_ex1 gstk_C13 2"
+value "multi_step tre0_ex1 gstk_C13 3"
 *)
 
-value "check_gs_gas_stp (multi_step tre0_ex1 gstk_C13 2 20) (3000000-(375+8*32+375*4))"
+value "check_gs_gas_stp (multi_step tre0_ex1 gstk_C13 2) (3000000-(375+8*32+375*4))"
 
-value "\<not> check_gstk_exc_stp (multi_step tre0_ex1 gstk_C13 3 20)"
+value "\<not> check_gstk_exc_stp (multi_step tre0_ex1 gstk_C13 3)"
 
 
 (*C14 --- 
    invalid()
 *)
 (*
-value "multi_step tre0_ex1 gstk_C14 1 20"
-value "multi_step tre0_ex1 gstk_C14 2 20"
+value "multi_step tre0_ex1 gstk_C14 1"
+value "multi_step tre0_ex1 gstk_C14 2"
 *)
 
-value "check_gstk_exc_stp (multi_step tre0_ex1 gstk_C14 2 20)"
+value "check_gstk_exc_stp (multi_step tre0_ex1 gstk_C14 2)"
 
 
 (*C15 ---
   stop()
 *)
 (*
-value "multi_step tre0_ex1 gstk_C15 1 20"
-value "multi_step tre0_ex1 gstk_C15 2 20"
+value "multi_step tre0_ex1 gstk_C15 1"
+value "multi_step tre0_ex1 gstk_C15 2"
 *)
 
-value "check_gs_gas_stp (multi_step tre0_ex1 gstk_C15 2 20) (3000000)"
+value "check_gs_gas_stp (multi_step tre0_ex1 gstk_C15 2) (3000000)"
 
-value "\<not> check_gstk_exc_stp (multi_step tre0_ex1 gstk_C15 2 20)"
+value "\<not> check_gstk_exc_stp (multi_step tre0_ex1 gstk_C15 2)"
 
 
 (*C16 --- external call fails.
@@ -315,39 +315,39 @@ value "\<not> check_gstk_exc_stp (multi_step tre0_ex1 gstk_C15 2 20)"
      callcodeblk{ }
 *)
 (*
-value "multi_step tre0_ex1 gstk_C16 1 10"
-value "multi_step tre0_ex1 gstk_C16 2 10"
-value "multi_step tre0_ex1 gstk_C16 3 10"
-value "multi_step tre0_ex1 gstk_C16 4 10"
-value "multi_step tre0_ex1 gstk_C16 5 10"
-value "multi_step tre0_ex1 gstk_C16 6 10"
+value "multi_step tre0_ex1 gstk_C16 1"
+value "multi_step tre0_ex1 gstk_C16 2"
+value "multi_step tre0_ex1 gstk_C16 3"
+value "multi_step tre0_ex1 gstk_C16 4"
+value "multi_step tre0_ex1 gstk_C16 5"
+value "multi_step tre0_ex1 gstk_C16 6"
 *)
 
-value "check_var_val_stp (multi_step tre0_ex1 gstk_C16 5 10)
+value "check_var_val_stp (multi_step tre0_ex1 gstk_C16 5)
   [(xx_id, (NL 0) :L U256),(y_id, (NL 400) :L U256)]" 
 
-value "check_gs_gas_stp (multi_step tre0_ex1 gstk_C16 6 10) (3000000-14)"
+value "check_gs_gas_stp (multi_step tre0_ex1 gstk_C16 6) (3000000-14)"
 
-value "check_gstk_exc_stp (multi_step tre0_ex1 gstk_C16 2 10)"
+value "check_gstk_exc_stp (multi_step tre0_ex1 gstk_C16 2)"
 
 
 (*C17 --- same code as C16, but to_addr is None and eternal call successes.*)
 (*
-value "multi_step tre0_ex1 gstk_C17 1 10"
-value "multi_step tre0_ex1 gstk_C17 2 10"
-value "multi_step tre0_ex1 gstk_C17 3 10"
-value "multi_step tre0_ex1 gstk_C17 4 10"
-value "multi_step tre0_ex1 gstk_C17 5 10"
-value "multi_step tre0_ex1 gstk_C17 6 10"
-value "multi_step tre0_ex1 gstk_C17 7 10"
+value "multi_step tre0_ex1 gstk_C17 1"
+value "multi_step tre0_ex1 gstk_C17 2"
+value "multi_step tre0_ex1 gstk_C17 3"
+value "multi_step tre0_ex1 gstk_C17 4"
+value "multi_step tre0_ex1 gstk_C17 5"
+value "multi_step tre0_ex1 gstk_C17 6"
+value "multi_step tre0_ex1 gstk_C17 7"
 *)
 
-value "check_var_val_stp (multi_step tre0_ex1 gstk_C17 6 10)
+value "check_var_val_stp (multi_step tre0_ex1 gstk_C17 6)
   [(xx_id, (NL 1) :L U256),(y_id, (NL 400) :L U256)]" 
 
-value "check_gs_gas_stp (multi_step tre0_ex1 gstk_C17 7 10) (3000000-9714)"
+value "check_gs_gas_stp (multi_step tre0_ex1 gstk_C17 7) (3000000-9714)"
 
-value "\<not> check_gstk_exc_stp (multi_step tre0_ex1 gstk_C17 3 10)"
+value "\<not> check_gstk_exc_stp (multi_step tre0_ex1 gstk_C17 3)"
 
 
 (*C18 --- external call fails and gas exhaustion. 
@@ -358,35 +358,35 @@ value "\<not> check_gstk_exc_stp (multi_step tre0_ex1 gstk_C17 3 10)"
      delegatecallblk{ }
 *)
 (*
-value "multi_step tre0_ex1 gstk_C18 1 10"
-value "multi_step tre0_ex1 gstk_C18 2 10"
-value "multi_step tre0_ex1 gstk_C18 3 10"
-value "multi_step tre0_ex1 gstk_C18 4 10"
-value "multi_step tre0_ex1 gstk_C18 5 10"
+value "multi_step tre0_ex1 gstk_C18 1"
+value "multi_step tre0_ex1 gstk_C18 2"
+value "multi_step tre0_ex1 gstk_C18 3"
+value "multi_step tre0_ex1 gstk_C18 4"
+value "multi_step tre0_ex1 gstk_C18 5"
 *)
 
-value "check_gstk_exc_stp (multi_step tre0_ex1 gstk_C18 2 10)"
+value "check_gstk_exc_stp (multi_step tre0_ex1 gstk_C18 2)"
 
-value "check_gstk_exc_stp (multi_step tre0_ex1 gstk_C18 5 10)"
+value "check_gstk_exc_stp (multi_step tre0_ex1 gstk_C18 5)"
 
 
 (*C19 --- same code as C18, but to_addr is None*)
 (*
-value "multi_step tre0_ex1 gstk_C19 1 10"
-value "multi_step tre0_ex1 gstk_C19 2 10"
-value "multi_step tre0_ex1 gstk_C19 3 10"
-value "multi_step tre0_ex1 gstk_C19 4 10"
-value "multi_step tre0_ex1 gstk_C19 5 10"
-value "multi_step tre0_ex1 gstk_C19 6 10"
-value "multi_step tre0_ex1 gstk_C19 7 10"
+value "multi_step tre0_ex1 gstk_C19 1"
+value "multi_step tre0_ex1 gstk_C19 2"
+value "multi_step tre0_ex1 gstk_C19 3"
+value "multi_step tre0_ex1 gstk_C19 4"
+value "multi_step tre0_ex1 gstk_C19 5"
+value "multi_step tre0_ex1 gstk_C19 6"
+value "multi_step tre0_ex1 gstk_C19 7"
 *)
 
-value "check_var_val_stp (multi_step tre0_ex1 gstk_C19 6 10)
+value "check_var_val_stp (multi_step tre0_ex1 gstk_C19 6)
   [(xx_id, (NL 1) :L U256),(y_id, (NL 400) :L U256)]" 
 
-value "check_gs_gas_stp (multi_step tre0_ex1 gstk_C19 7 10) (3000000-714)"
+value "check_gs_gas_stp (multi_step tre0_ex1 gstk_C19 7) (3000000-714)"
 
-value "\<not> check_gstk_exc_stp (multi_step tre0_ex1 gstk_C19 3 10)"
+value "\<not> check_gstk_exc_stp (multi_step tre0_ex1 gstk_C19 3)"
 
 
 (*C20 --- with insufficient gas and gas exhaustion
@@ -397,47 +397,47 @@ value "\<not> check_gstk_exc_stp (multi_step tre0_ex1 gstk_C19 3 10)"
      callee{ }
 *)
 (*
-value "multi_step tre0_ex1 gstk_C20 1 10"
-value "multi_step tre0_ex1 gstk_C20 2 10"
-value "multi_step tre0_ex1 gstk_C20 3 10"
-value "multi_step tre0_ex1 gstk_C20 4 10"
+value "multi_step tre0_ex1 gstk_C20 1"
+value "multi_step tre0_ex1 gstk_C20 2"
+value "multi_step tre0_ex1 gstk_C20 3"
+value "multi_step tre0_ex1 gstk_C20 4"
 *)
 
-value "check_gstk_exc_stp (multi_step tre0_ex1 gstk_C20 2 10)"
+value "check_gstk_exc_stp (multi_step tre0_ex1 gstk_C20 2)"
 
-value "check_gstk_exc_stp (multi_step tre0_ex1 gstk_C20 4 10)"
+value "check_gstk_exc_stp (multi_step tre0_ex1 gstk_C20 4)"
 
 
 (*C21 --- same code as C20, but to_addr is None*)
 (*
-value "multi_step tre0_ex1 gstk_C21 1 10"
-value "multi_step tre0_ex1 gstk_C21 2 10"
-value "multi_step tre0_ex1 gstk_C21 3 10"
-value "multi_step tre0_ex1 gstk_C21 4 10"
-value "multi_step tre0_ex1 gstk_C21 5 10"
-value "multi_step tre0_ex1 gstk_C21 6 10"
-value "multi_step tre0_ex1 gstk_C21 7 10"
+value "multi_step tre0_ex1 gstk_C21 1"
+value "multi_step tre0_ex1 gstk_C21 2"
+value "multi_step tre0_ex1 gstk_C21 3"
+value "multi_step tre0_ex1 gstk_C21 4"
+value "multi_step tre0_ex1 gstk_C21 5"
+value "multi_step tre0_ex1 gstk_C21 6"
+value "multi_step tre0_ex1 gstk_C21 7"
 *)
 
-value "check_var_val_stp (multi_step tre0_ex1 gstk_C21 6 10)
+value "check_var_val_stp (multi_step tre0_ex1 gstk_C21 6)
   [(xx_id, (NL 1) :L U256),(y_id, (NL 400) :L U256)]" 
 
-value "check_gs_gas_stp (multi_step tre0_ex1 gstk_C21 7 10) (3000000-34714)"
+value "check_gs_gas_stp (multi_step tre0_ex1 gstk_C21 7) (3000000-34714)"
 
-value "\<not> check_gstk_exc_stp (multi_step tre0_ex1 gstk_C21 7 10)"
+value "\<not> check_gstk_exc_stp (multi_step tre0_ex1 gstk_C21 7)"
 
 
 (*C22 --- to_addr is None.
   selfdestruct(0)
 *)
 (*
-value "multi_step tre0_ex1 gstk_C22 1 10"
-value "multi_step tre0_ex1 gstk_C22 2 10"
+value "multi_step tre0_ex1 gstk_C22 1"
+value "multi_step tre0_ex1 gstk_C22 2"
 *)
 
-value "check_gs_gas_stp (multi_step tre0_ex1 gstk_C22 2 10) (3000000-30000)"
+value "check_gs_gas_stp (multi_step tre0_ex1 gstk_C22 2) (3000000-30000)"
 
-value "\<not> check_gstk_exc_stp (multi_step tre0_ex1 gstk_C22 2 10)"
+value "\<not> check_gstk_exc_stp (multi_step tre0_ex1 gstk_C22 2)"
 
 
 (*C23 --- with overflow of call stacks.
@@ -449,48 +449,48 @@ value "\<not> check_gstk_exc_stp (multi_step tre0_ex1 gstk_C22 2 10)"
       }
 *)
 (*
-value "multi_step tre0_ex1 (gstk_C23 # []) 1 100"
-value "multi_step tre0_ex1 (gstk_C23 # []) 2 100"
-value "multi_step tre0_ex1 (gstk_C23 # []) 3 100"
-value "multi_step tre0_ex1 (gstk_C23 # []) 4 100"
-value "multi_step tre0_ex1 (gstk_C23 # []) 5 100"
-value "multi_step tre0_ex1 (gstk_C23 # []) 6 100"
-value "multi_step tre0_ex1 (gstk_C23 # []) 7 100"
-value "multi_step tre0_ex1 (gstk_C23 # []) 8 100"
-value "multi_step tre0_ex1 (gstk_C23 # []) 9 100"
-value "multi_step tre0_ex1 (gstk_C23 # []) 10 100"
-value "multi_step tre0_ex1 (gstk_C23 # []) 11 100"
-value "multi_step tre0_ex1 (gstk_C23 # []) 12 100"
-value "multi_step tre0_ex1 (gstk_C23 # []) 13 100"
-value "multi_step tre0_ex1 (gstk_C23 # []) 14 100"
-value "multi_step tre0_ex1 (gstk_C23 # []) 15 100"
-value "multi_step tre0_ex1 (gstk_C23 # []) 16 100"
-value "multi_step tre0_ex1 (gstk_C23 # []) 17 100"
-value "multi_step tre0_ex1 (gstk_C23 # []) 18 100"
-value "multi_step tre0_ex1 (gstk_C23 # []) 1120 100"
-value "multi_step tre0_ex1 (gstk_C23 # []) 2020 100"
-value "multi_step tre0_ex1 (gstk_C23 # []) 2030 100"
-value "multi_step tre0_ex1 (gstk_C23 # []) 2033 100"
-value "multi_step tre0_ex1 (gstk_C23 # []) 2035 100"
-value "multi_step tre0_ex1 (gstk_C23 # []) 2037 100"
-value "multi_step tre0_ex1 (gstk_C23 # []) 2040 100"
-value "multi_step tre0_ex1 (gstk_C23 # []) 2042 100"
-value "multi_step tre0_ex1 (gstk_C23 # []) 2044 100"
-value "multi_step tre0_ex1 (gstk_C23 # []) 2046 100"
-value "multi_step tre0_ex1 (gstk_C23 # []) 2047 100"
-value "multi_step tre0_ex1 (gstk_C23 # []) 2048 100"
-value "multi_step tre0_ex1 (gstk_C23 # []) 2049 100"
-value "multi_step tre0_ex1 (gstk_C23 # []) 2050 100"
-value "multi_step tre0_ex1 (gstk_C23 # []) 2051 100"
-value "multi_step tre0_ex1 (gstk_C23 # []) 2052 100"
-value "multi_step tre0_ex1 (gstk_C23 # []) 2053 100"
-value "multi_step tre0_ex1 (gstk_C23 # []) 2054 100"
-value "multi_step tre0_ex1 (gstk_C23 # []) 4210 100"
+value "multi_step tre0_ex1 (gstk_C23 # []) 1"
+value "multi_step tre0_ex1 (gstk_C23 # []) 2"
+value "multi_step tre0_ex1 (gstk_C23 # []) 3"
+value "multi_step tre0_ex1 (gstk_C23 # []) 4"
+value "multi_step tre0_ex1 (gstk_C23 # []) 5"
+value "multi_step tre0_ex1 (gstk_C23 # []) 6"
+value "multi_step tre0_ex1 (gstk_C23 # []) 7"
+value "multi_step tre0_ex1 (gstk_C23 # []) 8"
+value "multi_step tre0_ex1 (gstk_C23 # []) 9"
+value "multi_step tre0_ex1 (gstk_C23 # []) 10"
+value "multi_step tre0_ex1 (gstk_C23 # []) 11"
+value "multi_step tre0_ex1 (gstk_C23 # []) 12"
+value "multi_step tre0_ex1 (gstk_C23 # []) 13"
+value "multi_step tre0_ex1 (gstk_C23 # []) 14"
+value "multi_step tre0_ex1 (gstk_C23 # []) 15"
+value "multi_step tre0_ex1 (gstk_C23 # []) 16"
+value "multi_step tre0_ex1 (gstk_C23 # []) 17"
+value "multi_step tre0_ex1 (gstk_C23 # []) 18"
+value "multi_step tre0_ex1 (gstk_C23 # []) 1120"
+value "multi_step tre0_ex1 (gstk_C23 # []) 2020"
+value "multi_step tre0_ex1 (gstk_C23 # []) 2030"
+value "multi_step tre0_ex1 (gstk_C23 # []) 2033"
+value "multi_step tre0_ex1 (gstk_C23 # []) 2035"
+value "multi_step tre0_ex1 (gstk_C23 # []) 2037"
+value "multi_step tre0_ex1 (gstk_C23 # []) 2040"
+value "multi_step tre0_ex1 (gstk_C23 # []) 2042"
+value "multi_step tre0_ex1 (gstk_C23 # []) 2044"
+value "multi_step tre0_ex1 (gstk_C23 # []) 2046"
+value "multi_step tre0_ex1 (gstk_C23 # []) 2047"
+value "multi_step tre0_ex1 (gstk_C23 # []) 2048"
+value "multi_step tre0_ex1 (gstk_C23 # []) 2049"
+value "multi_step tre0_ex1 (gstk_C23 # []) 2050"
+value "multi_step tre0_ex1 (gstk_C23 # []) 2051"
+value "multi_step tre0_ex1 (gstk_C23 # []) 2052"
+value "multi_step tre0_ex1 (gstk_C23 # []) 2053"
+value "multi_step tre0_ex1 (gstk_C23 # []) 2054"
+value "multi_step tre0_ex1 (gstk_C23 # []) 4210"
 *)
 
-value "check_gstk_exc_stp (multi_step tre0_ex1 (gstk_C23 # []) 2048 100)"
+value "check_gstk_exc_stp (multi_step tre0_ex1 (gstk_C23 # []) 2048)"
 
-value "\<not> check_gstk_exc_stp (multi_step tre0_ex1 (gstk_C23 # []) 2049 100)"
+value "\<not> check_gstk_exc_stp (multi_step tre0_ex1 (gstk_C23 # []) 2049)"
 
 
 (*C24 --- with overflow of call stacks.
@@ -502,31 +502,31 @@ value "\<not> check_gstk_exc_stp (multi_step tre0_ex1 (gstk_C23 # []) 2049 100)"
       }
 *)
 (*
-value "multi_step tre0_ex1 (gstk_C24 # []) 1 100"
-value "multi_step tre0_ex1 (gstk_C24 # []) 2 100"
-value "multi_step tre0_ex1 (gstk_C24 # []) 3 100"
-value "multi_step tre0_ex1 (gstk_C24 # []) 4 100"
-value "multi_step tre0_ex1 (gstk_C24 # []) 5 100"
-value "multi_step tre0_ex1 (gstk_C24 # []) 6 100"
-value "multi_step tre0_ex1 (gstk_C24 # []) 7 100"
-value "multi_step tre0_ex1 (gstk_C24 # []) 8 100"
-value "multi_step tre0_ex1 (gstk_C24 # []) 9 100"
-value "multi_step tre0_ex1 (gstk_C24 # []) 10 100"
-value "multi_step tre0_ex1 (gstk_C24 # []) 2044 100"
-value "multi_step tre0_ex1 (gstk_C24 # []) 2046 100"
-value "multi_step tre0_ex1 (gstk_C24 # []) 2047 100"
-value "multi_step tre0_ex1 (gstk_C24 # []) 2048 100"
-value "multi_step tre0_ex1 (gstk_C24 # []) 2049 100"
-value "multi_step tre0_ex1 (gstk_C24 # []) 2050 100"
-value "multi_step tre0_ex1 (gstk_C24 # []) 2051 100"
-value "multi_step tre0_ex1 (gstk_C24 # []) 2052 100"
-value "multi_step tre0_ex1 (gstk_C24 # []) 2053 100"
-value "multi_step tre0_ex1 (gstk_C24 # []) 2054 100"
+value "multi_step tre0_ex1 (gstk_C24 # []) 1"
+value "multi_step tre0_ex1 (gstk_C24 # []) 2"
+value "multi_step tre0_ex1 (gstk_C24 # []) 3"
+value "multi_step tre0_ex1 (gstk_C24 # []) 4"
+value "multi_step tre0_ex1 (gstk_C24 # []) 5"
+value "multi_step tre0_ex1 (gstk_C24 # []) 6"
+value "multi_step tre0_ex1 (gstk_C24 # []) 7"
+value "multi_step tre0_ex1 (gstk_C24 # []) 8"
+value "multi_step tre0_ex1 (gstk_C24 # []) 9"
+value "multi_step tre0_ex1 (gstk_C24 # []) 10"
+value "multi_step tre0_ex1 (gstk_C24 # []) 2044"
+value "multi_step tre0_ex1 (gstk_C24 # []) 2046"
+value "multi_step tre0_ex1 (gstk_C24 # []) 2047"
+value "multi_step tre0_ex1 (gstk_C24 # []) 2048"
+value "multi_step tre0_ex1 (gstk_C24 # []) 2049"
+value "multi_step tre0_ex1 (gstk_C24 # []) 2050"
+value "multi_step tre0_ex1 (gstk_C24 # []) 2051"
+value "multi_step tre0_ex1 (gstk_C24 # []) 2052"
+value "multi_step tre0_ex1 (gstk_C24 # []) 2053"
+value "multi_step tre0_ex1 (gstk_C24 # []) 2054"
 *)
 
-value "check_gstk_exc_stp (multi_step tre0_ex1 (gstk_C24 # []) 2048 100)"
+value "check_gstk_exc_stp (multi_step tre0_ex1 (gstk_C24 # []) 2048)"
 
-value "\<not> check_gstk_exc_stp (multi_step tre0_ex1 (gstk_C24 # []) 2049 100)"
+value "\<not> check_gstk_exc_stp (multi_step tre0_ex1 (gstk_C24 # []) 2049)"
 
 
 end
