tests/TestsBuiltin_Logic.thy
@@ -24,76 +24,76 @@ begin
 (*L1 ---  (b=false, a=0) \<rightarrow>* (h=true)
       h := lor(b, eq(a,mul(0,3)))*)
 (*
-value "multi_step tre0_ex1 gstk_L1 1 10"
-value "multi_step tre0_ex1 gstk_L1 2 10"
-value "multi_step tre0_ex1 gstk_L1 3 10"
-value "multi_step tre0_ex1 gstk_L1 4 10"
-value "multi_step tre0_ex1 gstk_L1 5 10"
-value "multi_step tre0_ex1 gstk_L1 6 10"
-value "multi_step tre0_ex1 gstk_L1 7 10"
-value "multi_step tre0_ex1 gstk_L1 8 10"
-value "multi_step tre0_ex1 gstk_L1 9 10"
+value "multi_step tre0_ex1 gstk_L1 1"
+value "multi_step tre0_ex1 gstk_L1 2"
+value "multi_step tre0_ex1 gstk_L1 3"
+value "multi_step tre0_ex1 gstk_L1 4"
+value "multi_step tre0_ex1 gstk_L1 5"
+value "multi_step tre0_ex1 gstk_L1 6"
+value "multi_step tre0_ex1 gstk_L1 7"
+value "multi_step tre0_ex1 gstk_L1 8"
+value "multi_step tre0_ex1 gstk_L1 9"
 *)
 
-value "check_var_val_stp (multi_step tre0_ex1 gstk_L1 9 10) [(h_id, TL :L Bool)]"
+value "check_var_val_stp (multi_step tre0_ex1 gstk_L1 9) [(h_id, TL :L Bool)]"
 
-value "check_gs_gas_stp (multi_step tre0_ex1 gstk_L1 9 10) (3000000-3-3-5-3-3-5)"
+value "check_gs_gas_stp (multi_step tre0_ex1 gstk_L1 9) (3000000-3-3-5-3-3-5)"
 
-value "\<not> check_gstk_exc_stp (multi_step tre0_ex1 gstk_L1 9 10)"
+value "\<not> check_gstk_exc_stp (multi_step tre0_ex1 gstk_L1 9)"
 
 
 (*L2 --- (b=false, a=0) \<rightarrow>* (h=false)
     h := land(b, lt(a,3))*)
 (*
-value "multi_step tre0_ex1 gstk_L2 1 10"
-value "multi_step tre0_ex1 gstk_L2 2 10"
-value "multi_step tre0_ex1 gstk_L2 3 10"
-value "multi_step tre0_ex1 gstk_L2 4 10"
-value "multi_step tre0_ex1 gstk_L2 5 10"
-value "multi_step tre0_ex1 gstk_L2 6 10"
-value "multi_step tre0_ex1 gstk_L2 7 10"
+value "multi_step tre0_ex1 gstk_L2 1"
+value "multi_step tre0_ex1 gstk_L2 2"
+value "multi_step tre0_ex1 gstk_L2 3"
+value "multi_step tre0_ex1 gstk_L2 4"
+value "multi_step tre0_ex1 gstk_L2 5"
+value "multi_step tre0_ex1 gstk_L2 6"
+value "multi_step tre0_ex1 gstk_L2 7"
 *)
 
-value "check_var_val_stp (multi_step tre0_ex1 gstk_L2 7 10) [(h_id, FL :L Bool)]"
+value "check_var_val_stp (multi_step tre0_ex1 gstk_L2 7) [(h_id, FL :L Bool)]"
 
-value "check_gs_gas_stp (multi_step tre0_ex1 gstk_L2 7 10) (3000000-3-3-3-3-5)"
+value "check_gs_gas_stp (multi_step tre0_ex1 gstk_L2 7) (3000000-3-3-3-3-5)"
 
-value "\<not> check_gstk_exc_stp (multi_step tre0_ex1 gstk_L2 7 10)"
+value "\<not> check_gstk_exc_stp (multi_step tre0_ex1 gstk_L2 7)"
 
 
 (*L3 --- (b=false, x=0) \<rightarrow>* (h=false)
        h := lxor(b,gt(x,2))*)
 (*
-value "multi_step tre0_ex1 gstk_L3 1 10"
-value "multi_step tre0_ex1 gstk_L3 2 10"
-value "multi_step tre0_ex1 gstk_L3 3 10"
-value "multi_step tre0_ex1 gstk_L3 4 10"
-value "multi_step tre0_ex1 gstk_L3 5 10"   
-value "multi_step tre0_ex1 gstk_L3 6 10"
-value "multi_step tre0_ex1 gstk_L3 7 10"
+value "multi_step tre0_ex1 gstk_L3 1"
+value "multi_step tre0_ex1 gstk_L3 2"
+value "multi_step tre0_ex1 gstk_L3 3"
+value "multi_step tre0_ex1 gstk_L3 4"
+value "multi_step tre0_ex1 gstk_L3 5"   
+value "multi_step tre0_ex1 gstk_L3 6"
+value "multi_step tre0_ex1 gstk_L3 7"
 *)
 
-value "check_var_val_stp (multi_step tre0_ex1 gstk_L3 7 10) [(h_id, FL :L Bool)]"
+value "check_var_val_stp (multi_step tre0_ex1 gstk_L3 7) [(h_id, FL :L Bool)]"
 
-value "check_gs_gas_stp (multi_step tre0_ex1 gstk_L3 7 10) (3000000-3-3-3-3-5)"
+value "check_gs_gas_stp (multi_step tre0_ex1 gstk_L3 7) (3000000-3-3-3-3-5)"
 
-value "\<not> check_gstk_exc_stp (multi_step tre0_ex1 gstk_L3 7 10)"
+value "\<not> check_gstk_exc_stp (multi_step tre0_ex1 gstk_L3 7)"
 
 
 (*L4 --- (b=false) \<rightarrow>* (h=true)
       h := lnot(b)*)
 (*
-value "multi_step tre0_ex1 gstk_L4 1 10"
-value "multi_step tre0_ex1 gstk_L4 2 10"
-value "multi_step tre0_ex1 gstk_L4 3 10"
-value "multi_step tre0_ex1 gstk_L4 4 10"
+value "multi_step tre0_ex1 gstk_L4 1"
+value "multi_step tre0_ex1 gstk_L4 2"
+value "multi_step tre0_ex1 gstk_L4 3"
+value "multi_step tre0_ex1 gstk_L4 4"
 *)
 
-value "check_var_val_stp (multi_step tre0_ex1 gstk_L4 4 10) [(h_id, TL :L Bool)]"
+value "check_var_val_stp (multi_step tre0_ex1 gstk_L4 4) [(h_id, TL :L Bool)]"
 
-value "check_gs_gas_stp (multi_step tre0_ex1 gstk_L4 4 10) (3000000-3-3-5)"
+value "check_gs_gas_stp (multi_step tre0_ex1 gstk_L4 4) (3000000-3-3-5)"
 
-value "\<not> check_gstk_exc_stp (multi_step tre0_ex1 gstk_L4 4 10)"
+value "\<not> check_gstk_exc_stp (multi_step tre0_ex1 gstk_L4 4)"
 
 
 (*L5 --- (b=false) \<rightarrow>* (b=true)
@@ -101,69 +101,69 @@ value "\<not> check_gstk_exc_stp (multi_step tre0_ex1 gstk_L4 4 10)"
   b := lor(f3(), b)
 *)
 (*
-value "multi_step tre0_ex1 gstk_L5 1 20"
-value "multi_step tre0_ex1 gstk_L5 2 20"
-value "multi_step tre0_ex1 gstk_L5 3 20"
-value "multi_step tre0_ex1 gstk_L5 4 20"
-value "multi_step tre0_ex1 gstk_L5 5 20"
-value "multi_step tre0_ex1 gstk_L5 6 20"
-value "multi_step tre0_ex1 gstk_L5 7 20"
-value "multi_step tre0_ex1 gstk_L5 8 20"
-value "multi_step tre0_ex1 gstk_L5 9 20"
-value "multi_step tre0_ex1 gstk_L5 10 20"
-value "multi_step tre0_ex1 gstk_L5 11 20"
-value "multi_step tre0_ex1 gstk_L5 12 20"
-value "multi_step tre0_ex1 gstk_L5 13 20"
-value "multi_step tre0_ex1 gstk_L5 14 20"
-value "multi_step tre0_ex1 gstk_L5 15 20"
-value "multi_step tre0_ex1 gstk_L5 16 20"
-value "multi_step tre0_ex1 gstk_L5 17 20"
-value "multi_step tre0_ex1 gstk_L5 18 20"
-value "multi_step tre0_ex1 gstk_L5 19 20"
-value "multi_step tre0_ex1 gstk_L5 20 20"
-value "multi_step tre0_ex1 gstk_L5 21 20"
-value "multi_step tre0_ex1 gstk_L5 22 20"
+value "multi_step tre0_ex1 gstk_L5 1"
+value "multi_step tre0_ex1 gstk_L5 2"
+value "multi_step tre0_ex1 gstk_L5 3"
+value "multi_step tre0_ex1 gstk_L5 4"
+value "multi_step tre0_ex1 gstk_L5 5"
+value "multi_step tre0_ex1 gstk_L5 6"
+value "multi_step tre0_ex1 gstk_L5 7"
+value "multi_step tre0_ex1 gstk_L5 8"
+value "multi_step tre0_ex1 gstk_L5 9"
+value "multi_step tre0_ex1 gstk_L5 10"
+value "multi_step tre0_ex1 gstk_L5 11"
+value "multi_step tre0_ex1 gstk_L5 12"
+value "multi_step tre0_ex1 gstk_L5 13"
+value "multi_step tre0_ex1 gstk_L5 14"
+value "multi_step tre0_ex1 gstk_L5 15"
+value "multi_step tre0_ex1 gstk_L5 16"
+value "multi_step tre0_ex1 gstk_L5 17"
+value "multi_step tre0_ex1 gstk_L5 18"
+value "multi_step tre0_ex1 gstk_L5 19"
+value "multi_step tre0_ex1 gstk_L5 20"
+value "multi_step tre0_ex1 gstk_L5 21"
+value "multi_step tre0_ex1 gstk_L5 22"
 *)
 
-value "check_var_val_stp (multi_step tre0_ex1 gstk_L5 21 20) [(b_id, TL :L Bool)]"
+value "check_var_val_stp (multi_step tre0_ex1 gstk_L5 21) [(b_id, TL :L Bool)]"
 
-value "check_gs_gas_stp (multi_step tre0_ex1 gstk_L5 22 20) (3000000-72)"
+value "check_gs_gas_stp (multi_step tre0_ex1 gstk_L5 22) (3000000-72)"
 
-value "\<not> check_gstk_exc_stp (multi_step tre0_ex1 gstk_L5 22 20)"
+value "\<not> check_gstk_exc_stp (multi_step tre0_ex1 gstk_L5 22)"
 
 
 (*L6 --- same code as L5, but with gas exhaustion*)
 (*
-value "multi_step tre0_ex1 gstk_L6 1 20"
-value "multi_step tre0_ex1 gstk_L6 2 20"
-value "multi_step tre0_ex1 gstk_L6 3 20"
-value "multi_step tre0_ex1 gstk_L6 4 20"
-value "multi_step tre0_ex1 gstk_L6 5 20"
-value "multi_step tre0_ex1 gstk_L6 6 20"
-value "multi_step tre0_ex1 gstk_L6 7 20"
-value "multi_step tre0_ex1 gstk_L6 8 20"
-value "multi_step tre0_ex1 gstk_L6 9 20"
-value "multi_step tre0_ex1 gstk_L6 10 20"
-value "multi_step tre0_ex1 gstk_L6 11 20"
-value "multi_step tre0_ex1 gstk_L6 12 20"
-value "multi_step tre0_ex1 gstk_L6 13 20"
-value "multi_step tre0_ex1 gstk_L6 14 20"
-value "multi_step tre0_ex1 gstk_L6 15 20"
-value "multi_step tre0_ex1 gstk_L6 16 20"
-value "multi_step tre0_ex1 gstk_L6 17 20"
+value "multi_step tre0_ex1 gstk_L6 1"
+value "multi_step tre0_ex1 gstk_L6 2"
+value "multi_step tre0_ex1 gstk_L6 3"
+value "multi_step tre0_ex1 gstk_L6 4"
+value "multi_step tre0_ex1 gstk_L6 5"
+value "multi_step tre0_ex1 gstk_L6 6"
+value "multi_step tre0_ex1 gstk_L6 7"
+value "multi_step tre0_ex1 gstk_L6 8"
+value "multi_step tre0_ex1 gstk_L6 9"
+value "multi_step tre0_ex1 gstk_L6 10"
+value "multi_step tre0_ex1 gstk_L6 11"
+value "multi_step tre0_ex1 gstk_L6 12"
+value "multi_step tre0_ex1 gstk_L6 13"
+value "multi_step tre0_ex1 gstk_L6 14"
+value "multi_step tre0_ex1 gstk_L6 15"
+value "multi_step tre0_ex1 gstk_L6 16"
+value "multi_step tre0_ex1 gstk_L6 17"
 *)
 
-value "check_gstk_exc_stp (multi_step tre0_ex1 gstk_L6 17 20)"
+value "check_gstk_exc_stp (multi_step tre0_ex1 gstk_L6 17)"
 
 
 (*L7 --- same code as L5, but with overflow of words stack*)
 (*
-value "multi_step tre0_ex1 gstk_L7 1 20"
-value "multi_step tre0_ex1 gstk_L7 2 20"
-value "multi_step tre0_ex1 gstk_L7 3 20"
+value "multi_step tre0_ex1 gstk_L7 1"
+value "multi_step tre0_ex1 gstk_L7 2"
+value "multi_step tre0_ex1 gstk_L7 3"
 *)
 
-value "check_gstk_exc_stp (multi_step tre0_ex1 gstk_L7 3 20)"
+value "check_gstk_exc_stp (multi_step tre0_ex1 gstk_L7 3)"
 
 
 (*L8 --- (b=false) \<rightarrow>* (b=true)
@@ -171,92 +171,92 @@ value "check_gstk_exc_stp (multi_step tre0_ex1 gstk_L7 3 20)"
   b := lxor(f3(), not(f3()))
 *)
 (*
-value "multi_step tre0_ex1 gstk_L8 1 20"
-value "multi_step tre0_ex1 gstk_L8 2 20"
-value "multi_step tre0_ex1 gstk_L8 3 20"
-value "multi_step tre0_ex1 gstk_L8 4 20"
-value "multi_step tre0_ex1 gstk_L8 5 20"
-value "multi_step tre0_ex1 gstk_L8 6 20"
-value "multi_step tre0_ex1 gstk_L8 7 20"
-value "multi_step tre0_ex1 gstk_L8 8 20"
-value "multi_step tre0_ex1 gstk_L8 9 20"
-value "multi_step tre0_ex1 gstk_L8 10 20"
-value "multi_step tre0_ex1 gstk_L8 11 20"
-value "multi_step tre0_ex1 gstk_L8 12 20"
-value "multi_step tre0_ex1 gstk_L8 13 20"
-value "multi_step tre0_ex1 gstk_L8 14 20"
-value "multi_step tre0_ex1 gstk_L8 15 20"
-value "multi_step tre0_ex1 gstk_L8 16 20"
-value "multi_step tre0_ex1 gstk_L8 17 20"
-value "multi_step tre0_ex1 gstk_L8 18 20"
-value "multi_step tre0_ex1 gstk_L8 19 20"
-value "multi_step tre0_ex1 gstk_L8 20 20"
-value "multi_step tre0_ex1 gstk_L8 21 20"
-value "multi_step tre0_ex1 gstk_L8 22 20"
-value "multi_step tre0_ex1 gstk_L8 23 20"
-value "multi_step tre0_ex1 gstk_L8 24 20"
-value "multi_step tre0_ex1 gstk_L8 25 20"
-value "multi_step tre0_ex1 gstk_L8 26 20"
-value "multi_step tre0_ex1 gstk_L8 27 20"
-value "multi_step tre0_ex1 gstk_L8 28 20"
-value "multi_step tre0_ex1 gstk_L8 29 20"
-value "multi_step tre0_ex1 gstk_L8 30 20"
-value "multi_step tre0_ex1 gstk_L8 31 20"
-value "multi_step tre0_ex1 gstk_L8 32 20"
-value "multi_step tre0_ex1 gstk_L8 33 20"
-value "multi_step tre0_ex1 gstk_L8 34 20"
-value "multi_step tre0_ex1 gstk_L8 35 20"
-value "multi_step tre0_ex1 gstk_L8 36 20"
+value "multi_step tre0_ex1 gstk_L8 1"
+value "multi_step tre0_ex1 gstk_L8 2"
+value "multi_step tre0_ex1 gstk_L8 3"
+value "multi_step tre0_ex1 gstk_L8 4"
+value "multi_step tre0_ex1 gstk_L8 5"
+value "multi_step tre0_ex1 gstk_L8 6"
+value "multi_step tre0_ex1 gstk_L8 7"
+value "multi_step tre0_ex1 gstk_L8 8"
+value "multi_step tre0_ex1 gstk_L8 9"
+value "multi_step tre0_ex1 gstk_L8 10"
+value "multi_step tre0_ex1 gstk_L8 11"
+value "multi_step tre0_ex1 gstk_L8 12"
+value "multi_step tre0_ex1 gstk_L8 13"
+value "multi_step tre0_ex1 gstk_L8 14"
+value "multi_step tre0_ex1 gstk_L8 15"
+value "multi_step tre0_ex1 gstk_L8 16"
+value "multi_step tre0_ex1 gstk_L8 17"
+value "multi_step tre0_ex1 gstk_L8 18"
+value "multi_step tre0_ex1 gstk_L8 19"
+value "multi_step tre0_ex1 gstk_L8 20"
+value "multi_step tre0_ex1 gstk_L8 21"
+value "multi_step tre0_ex1 gstk_L8 22"
+value "multi_step tre0_ex1 gstk_L8 23"
+value "multi_step tre0_ex1 gstk_L8 24"
+value "multi_step tre0_ex1 gstk_L8 25"
+value "multi_step tre0_ex1 gstk_L8 26"
+value "multi_step tre0_ex1 gstk_L8 27"
+value "multi_step tre0_ex1 gstk_L8 28"
+value "multi_step tre0_ex1 gstk_L8 29"
+value "multi_step tre0_ex1 gstk_L8 30"
+value "multi_step tre0_ex1 gstk_L8 31"
+value "multi_step tre0_ex1 gstk_L8 32"
+value "multi_step tre0_ex1 gstk_L8 33"
+value "multi_step tre0_ex1 gstk_L8 34"
+value "multi_step tre0_ex1 gstk_L8 35"
+value "multi_step tre0_ex1 gstk_L8 36"
 *)
 
-value "check_var_val_stp (multi_step tre0_ex1 gstk_L8 35 20) [(b_id, TL :L Bool)]"
+value "check_var_val_stp (multi_step tre0_ex1 gstk_L8 35) [(b_id, TL :L Bool)]"
 
-value "check_gs_gas_stp (multi_step tre0_ex1 gstk_L8 36 20) (3000000-116)"
+value "check_gs_gas_stp (multi_step tre0_ex1 gstk_L8 36) (3000000-116)"
 
-value "\<not> check_gstk_exc_stp (multi_step tre0_ex1 gstk_L8 36 20)"
+value "\<not> check_gstk_exc_stp (multi_step tre0_ex1 gstk_L8 36)"
 
 
 (*L9 --- same code as L8, but with gas exhaustion*)
 (*
-value "multi_step tre0_ex1 gstk_L9 1 20"
-value "multi_step tre0_ex1 gstk_L9 2 20"
-value "multi_step tre0_ex1 gstk_L9 3 20"
-value "multi_step tre0_ex1 gstk_L9 4 20"
-value "multi_step tre0_ex1 gstk_L9 5 20"
-value "multi_step tre0_ex1 gstk_L9 6 20"
-value "multi_step tre0_ex1 gstk_L9 7 20"
-value "multi_step tre0_ex1 gstk_L9 8 20"
-value "multi_step tre0_ex1 gstk_L9 9 20"
-value "multi_step tre0_ex1 gstk_L9 10 20"
-value "multi_step tre0_ex1 gstk_L9 11 20"
-value "multi_step tre0_ex1 gstk_L9 12 20"
-value "multi_step tre0_ex1 gstk_L9 13 20"
-value "multi_step tre0_ex1 gstk_L9 14 20"
-value "multi_step tre0_ex1 gstk_L9 15 20"
-value "multi_step tre0_ex1 gstk_L9 16 20"
-value "multi_step tre0_ex1 gstk_L9 17 20"
-value "multi_step tre0_ex1 gstk_L9 18 20"
+value "multi_step tre0_ex1 gstk_L9 1"
+value "multi_step tre0_ex1 gstk_L9 2"
+value "multi_step tre0_ex1 gstk_L9 3"
+value "multi_step tre0_ex1 gstk_L9 4"
+value "multi_step tre0_ex1 gstk_L9 5"
+value "multi_step tre0_ex1 gstk_L9 6"
+value "multi_step tre0_ex1 gstk_L9 7"
+value "multi_step tre0_ex1 gstk_L9 8"
+value "multi_step tre0_ex1 gstk_L9 9"
+value "multi_step tre0_ex1 gstk_L9 10"
+value "multi_step tre0_ex1 gstk_L9 11"
+value "multi_step tre0_ex1 gstk_L9 12"
+value "multi_step tre0_ex1 gstk_L9 13"
+value "multi_step tre0_ex1 gstk_L9 14"
+value "multi_step tre0_ex1 gstk_L9 15"
+value "multi_step tre0_ex1 gstk_L9 16"
+value "multi_step tre0_ex1 gstk_L9 17"
+value "multi_step tre0_ex1 gstk_L9 18"
 *)
 
-value "check_gstk_exc_stp (multi_step tre0_ex1 gstk_L9 18 20)"
+value "check_gstk_exc_stp (multi_step tre0_ex1 gstk_L9 18)"
 
 
 (*L10 --- same code as L8, but with overflow of words stack*)
 (*
-value "multi_step tre0_ex1 gstk_L10 1 20"
-value "multi_step tre0_ex1 gstk_L10 2 20"
-value "multi_step tre0_ex1 gstk_L10 3 20"
-value "multi_step tre0_ex1 gstk_L10 4 20"
-value "multi_step tre0_ex1 gstk_L10 5 20"
-value "multi_step tre0_ex1 gstk_L10 6 20"
-value "multi_step tre0_ex1 gstk_L10 7 20"
-value "multi_step tre0_ex1 gstk_L10 8 20"
-value "multi_step tre0_ex1 gstk_L10 9 20"
-value "multi_step tre0_ex1 gstk_L10 10 20"
-value "multi_step tre0_ex1 gstk_L10 11 20"
+value "multi_step tre0_ex1 gstk_L10 1"
+value "multi_step tre0_ex1 gstk_L10 2"
+value "multi_step tre0_ex1 gstk_L10 3"
+value "multi_step tre0_ex1 gstk_L10 4"
+value "multi_step tre0_ex1 gstk_L10 5"
+value "multi_step tre0_ex1 gstk_L10 6"
+value "multi_step tre0_ex1 gstk_L10 7"
+value "multi_step tre0_ex1 gstk_L10 8"
+value "multi_step tre0_ex1 gstk_L10 9"
+value "multi_step tre0_ex1 gstk_L10 10"
+value "multi_step tre0_ex1 gstk_L10 11"
 *)
 
-value "check_gstk_exc_stp (multi_step tre0_ex1 gstk_L10 11 20)"
+value "check_gstk_exc_stp (multi_step tre0_ex1 gstk_L10 11)"
 
 
 end
