tests/TestsBuiltin_MemSto.thy
@@ -27,20 +27,20 @@ begin
   }
 *)
 (*
-value "multi_step tre0_ex1 gstk_M1 1 20"
-value "multi_step tre0_ex1 gstk_M1 2 20"
-value "multi_step tre0_ex1 gstk_M1 3 20"
-value "multi_step tre0_ex1 gstk_M1 4 20"
-value "multi_step tre0_ex1 gstk_M1 5 20"
-value "multi_step tre0_ex1 gstk_M1 6 20"
+value "multi_step tre0_ex1 gstk_M1 1"
+value "multi_step tre0_ex1 gstk_M1 2"
+value "multi_step tre0_ex1 gstk_M1 3"
+value "multi_step tre0_ex1 gstk_M1 4"
+value "multi_step tre0_ex1 gstk_M1 5"
+value "multi_step tre0_ex1 gstk_M1 6"
 *)
 
-value "check_var_val_stp (multi_step tre0_ex1 gstk_M1 5 20)
+value "check_var_val_stp (multi_step tre0_ex1 gstk_M1 5)
   [(x_id, (NL 11289525020298692601998108039226097635691122580326809888208074282503241728) :L U256)]" 
 
-value "check_gs_gas_stp (multi_step tre0_ex1 gstk_M1 6 20) (3000000-3-3-5-2)"
+value "check_gs_gas_stp (multi_step tre0_ex1 gstk_M1 6) (3000000-3-3-5-2)"
 
-value "\<not> check_gstk_exc_stp (multi_step tre0_ex1 gstk_M1 6 20)"
+value "\<not> check_gstk_exc_stp (multi_step tre0_ex1 gstk_M1 6)"
 
 
 (*M2 ---
@@ -48,21 +48,21 @@ value "\<not> check_gstk_exc_stp (multi_step tre0_ex1 gstk_M1 6 20)"
     x := mload(0x01)  
 *)
 (*
-value "multi_step tre0_ex1 gstk_M2 1 20"
-value "multi_step tre0_ex1 gstk_M2 2 20"
-value "multi_step tre0_ex1 gstk_M2 3 20"
-value "multi_step tre0_ex1 gstk_M2 4 20"
-value "multi_step tre0_ex1 gstk_M2 5 20"
-value "multi_step tre0_ex1 gstk_M2 6 20"
+value "multi_step tre0_ex1 gstk_M2 1"
+value "multi_step tre0_ex1 gstk_M2 2"
+value "multi_step tre0_ex1 gstk_M2 3"
+value "multi_step tre0_ex1 gstk_M2 4"
+value "multi_step tre0_ex1 gstk_M2 5"
+value "multi_step tre0_ex1 gstk_M2 6"
 *)
 
-value "check_var_val_stp (multi_step tre0_ex1 gstk_M2 5 20)
+value "check_var_val_stp (multi_step tre0_ex1 gstk_M2 5)
   [(x_id, 
     (NL 7691092201792325725438170817979025252018668099114851189875736584839327973633) :L U256)]" 
 
-value "check_gs_gas_stp (multi_step tre0_ex1 gstk_M2 6 20) (3000000-3-3-5-2)"
+value "check_gs_gas_stp (multi_step tre0_ex1 gstk_M2 6) (3000000-3-3-5-2)"
 
-value "\<not> check_gstk_exc_stp (multi_step tre0_ex1 gstk_M2 6 20)"
+value "\<not> check_gstk_exc_stp (multi_step tre0_ex1 gstk_M2 6)"
 
 
 (*M3 ---
@@ -70,19 +70,19 @@ value "\<not> check_gstk_exc_stp (multi_step tre0_ex1 gstk_M2 6 20)"
     x := sload(0x01)  
 *)
 (*
-value "multi_step tre0_ex1 gstk_M3 1 20"
-value "multi_step tre0_ex1 gstk_M3 2 20"
-value "multi_step tre0_ex1 gstk_M3 3 20"
-value "multi_step tre0_ex1 gstk_M3 4 20"
-value "multi_step tre0_ex1 gstk_M3 5 20"
-value "multi_step tre0_ex1 gstk_M3 6 20"
+value "multi_step tre0_ex1 gstk_M3 1"
+value "multi_step tre0_ex1 gstk_M3 2"
+value "multi_step tre0_ex1 gstk_M3 3"
+value "multi_step tre0_ex1 gstk_M3 4"
+value "multi_step tre0_ex1 gstk_M3 5"
+value "multi_step tre0_ex1 gstk_M3 6"
 *)
 
-value "check_var_val_stp (multi_step tre0_ex1 gstk_M3 5 20) [(x_id, (NL 17) :L U256)]" 
+value "check_var_val_stp (multi_step tre0_ex1 gstk_M3 5) [(x_id, (NL 17) :L U256)]" 
 
-value "check_gs_gas_stp (multi_step tre0_ex1 gstk_M3 6 20) (3000000-20000-200-5-2)"
+value "check_gs_gas_stp (multi_step tre0_ex1 gstk_M3 6) (3000000-20000-200-5-2)"
 
-value "\<not> check_gstk_exc_stp (multi_step tre0_ex1 gstk_M3 6 20)"
+value "\<not> check_gstk_exc_stp (multi_step tre0_ex1 gstk_M3 6)"
 
 
 (*M4 ---
@@ -91,17 +91,17 @@ value "\<not> check_gstk_exc_stp (multi_step tre0_ex1 gstk_M3 6 20)"
   }
 *)
 (*
-value "multi_step tre0_ex1 gstk_M4 1 20"
-value "multi_step tre0_ex1 gstk_M4 2 20"
-value "multi_step tre0_ex1 gstk_M4 3 20"
-value "multi_step tre0_ex1 gstk_M4 4 20"
+value "multi_step tre0_ex1 gstk_M4 1"
+value "multi_step tre0_ex1 gstk_M4 2"
+value "multi_step tre0_ex1 gstk_M4 3"
+value "multi_step tre0_ex1 gstk_M4 4"
 *)
 
-value "check_var_val_stp (multi_step tre0_ex1 gstk_M4 3 20) [(a1_id, (NL 96) :L U256)]" 
+value "check_var_val_stp (multi_step tre0_ex1 gstk_M4 3) [(a1_id, (NL 96) :L U256)]" 
 
-value "check_gs_gas_stp (multi_step tre0_ex1 gstk_M4 4 20) (3000000-2-5-2)"
+value "check_gs_gas_stp (multi_step tre0_ex1 gstk_M4 4) (3000000-2-5-2)"
 
-value "\<not> check_gstk_exc_stp (multi_step tre0_ex1 gstk_M4 4 20)"
+value "\<not> check_gstk_exc_stp (multi_step tre0_ex1 gstk_M4 4)"
 
 
 (*M5 --- (xx=0) \<rightarrow>* (xx=9)
@@ -112,103 +112,102 @@ value "\<not> check_gstk_exc_stp (multi_step tre0_ex1 gstk_M4 4 20)"
   }
 *)
 (*
-value "multi_step tre0_ex1 gstk_M5 1 20"
-value "multi_step tre0_ex1 gstk_M5 2 20"
-value "multi_step tre0_ex1 gstk_M5 3 20"
-value "multi_step tre0_ex1 gstk_M5 4 20"
-value "multi_step tre0_ex1 gstk_M5 5 20"
-value "multi_step tre0_ex1 gstk_M5 6 20"
-value "multi_step tre0_ex1 gstk_M5 7 20"
-value "multi_step tre0_ex1 gstk_M5 8 20"
-value "multi_step tre0_ex1 gstk_M5 9 20"
-value "multi_step tre0_ex1 gstk_M5 10 20"
-value "multi_step tre0_ex1 gstk_M5 11 20"
-value "multi_step tre0_ex1 gstk_M5 12 20"
-value "multi_step tre0_ex1 gstk_M5 13 20"
-value "multi_step tre0_ex1 gstk_M5 14 20"
-value "multi_step tre0_ex1 gstk_M5 15 20"
-value "multi_step tre0_ex1 gstk_M5 16 20"
-value "multi_step tre0_ex1 gstk_M5 17 20"
-value "multi_step tre0_ex1 gstk_M5 18 20"
-value "multi_step tre0_ex1 gstk_M5 19 20"
-value "multi_step tre0_ex1 gstk_M5 20 20"
-value "multi_step tre0_ex1 gstk_M5 21 20"
-value "multi_step tre0_ex1 gstk_M5 22 20"
-value "multi_step tre0_ex1 gstk_M5 23 20"
-value "multi_step tre0_ex1 gstk_M5 24 20"
-value "multi_step tre0_ex1 gstk_M5 25 20"
-value "multi_step tre0_ex1 gstk_M5 26 20"
-value "multi_step tre0_ex1 gstk_M5 27 20"
-value "multi_step tre0_ex1 gstk_M5 28 20"
-value "multi_step tre0_ex1 gstk_M5 29 20"
-value "multi_step tre0_ex1 gstk_M5 30 20"
-value "multi_step tre0_ex1 gstk_M5 31 20"
-value "multi_step tre0_ex1 gstk_M5 32 20"
-value "multi_step tre0_ex1 gstk_M5 33 20"
-value "multi_step tre0_ex1 gstk_M5 34 20"
-value "multi_step tre0_ex1 gstk_M5 35 20"
-value "multi_step tre0_ex1 gstk_M5 36 20"
-value "multi_step tre0_ex1 gstk_M5 37 20"
-value "multi_step tre0_ex1 gstk_M5 38 20"
-value "multi_step tre0_ex1 gstk_M5 39 20"
-value "multi_step tre0_ex1 gstk_M5 40 20"
-value "multi_step tre0_ex1 gstk_M5 41 20"
-value "multi_step tre0_ex1 gstk_M5 42 20"
-value "multi_step tre0_ex1 gstk_M5 43 20"
-value "multi_step tre0_ex1 gstk_M5 44 20"
-value "multi_step tre0_ex1 gstk_M5 45 20"
-value "multi_step tre0_ex1 gstk_M5 46 20"
-value "multi_step tre0_ex1 gstk_M5 47 20"
-value "multi_step tre0_ex1 gstk_M5 48 20"
-value "multi_step tre0_ex1 gstk_M5 49 20"
-value "multi_step tre0_ex1 gstk_M5 50 20"
+value "multi_step tre0_ex1 gstk_M5 1"
+value "multi_step tre0_ex1 gstk_M5 2"
+value "multi_step tre0_ex1 gstk_M5 3"
+value "multi_step tre0_ex1 gstk_M5 4"
+value "multi_step tre0_ex1 gstk_M5 5"
+value "multi_step tre0_ex1 gstk_M5 6"
+value "multi_step tre0_ex1 gstk_M5 7"
+value "multi_step tre0_ex1 gstk_M5 8"
+value "multi_step tre0_ex1 gstk_M5 9"
+value "multi_step tre0_ex1 gstk_M5 10"
+value "multi_step tre0_ex1 gstk_M5 11"
+value "multi_step tre0_ex1 gstk_M5 12"
+value "multi_step tre0_ex1 gstk_M5 13"
+value "multi_step tre0_ex1 gstk_M5 14"
+value "multi_step tre0_ex1 gstk_M5 15"
+value "multi_step tre0_ex1 gstk_M5 16"
+value "multi_step tre0_ex1 gstk_M5 17"
+value "multi_step tre0_ex1 gstk_M5 18"
+value "multi_step tre0_ex1 gstk_M5 19"
+value "multi_step tre0_ex1 gstk_M5 20"
+value "multi_step tre0_ex1 gstk_M5 21"
+value "multi_step tre0_ex1 gstk_M5 22"
+value "multi_step tre0_ex1 gstk_M5 23"
+value "multi_step tre0_ex1 gstk_M5 24"
+value "multi_step tre0_ex1 gstk_M5 25"
+value "multi_step tre0_ex1 gstk_M5 26"
+value "multi_step tre0_ex1 gstk_M5 27"
+value "multi_step tre0_ex1 gstk_M5 28"
+value "multi_step tre0_ex1 gstk_M5 29"
+value "multi_step tre0_ex1 gstk_M5 30"
+value "multi_step tre0_ex1 gstk_M5 31"
+value "multi_step tre0_ex1 gstk_M5 32"
+value "multi_step tre0_ex1 gstk_M5 33"
+value "multi_step tre0_ex1 gstk_M5 34"
+value "multi_step tre0_ex1 gstk_M5 35"
+value "multi_step tre0_ex1 gstk_M5 36"
+value "multi_step tre0_ex1 gstk_M5 37"
+value "multi_step tre0_ex1 gstk_M5 38"
+value "multi_step tre0_ex1 gstk_M5 39"
+value "multi_step tre0_ex1 gstk_M5 40"
+value "multi_step tre0_ex1 gstk_M5 41"
+value "multi_step tre0_ex1 gstk_M5 42"
+value "multi_step tre0_ex1 gstk_M5 43"
+value "multi_step tre0_ex1 gstk_M5 44"
+value "multi_step tre0_ex1 gstk_M5 45"
+value "multi_step tre0_ex1 gstk_M5 46"
+value "multi_step tre0_ex1 gstk_M5 47"
+value "multi_step tre0_ex1 gstk_M5 48"
+value "multi_step tre0_ex1 gstk_M5 49"
+value "multi_step tre0_ex1 gstk_M5 50"
 *)
 
-value "check_var_val_stp (multi_step tre0_ex1 gstk_M5 49 20) [(xx_id, (NL 20) :L U256)]" 
+value "check_var_val_stp (multi_step tre0_ex1 gstk_M5 49) [(xx_id, (NL 20) :L U256)]" 
 
-value "check_gs_gas_stp (multi_step tre0_ex1 gstk_M5 50 20) (3000000-183)"
+value "check_gs_gas_stp (multi_step tre0_ex1 gstk_M5 50) (3000000-183)"
 
-value "\<not> check_gstk_exc_stp (multi_step tre0_ex1 gstk_M5 50 20)"
+value "\<not> check_gstk_exc_stp (multi_step tre0_ex1 gstk_M5 50)"
 
 
 (*M6 --- same code as M5, but with gas exhaustion*)
 (*
-value "multi_step tre0_ex1 gstk_M6 1 20"
-value "multi_step tre0_ex1 gstk_M6 2 20"
-value "multi_step tre0_ex1 gstk_M6 3 20"
-value "multi_step tre0_ex1 gstk_M6 4 20"
-value "multi_step tre0_ex1 gstk_M6 5 20"
-value "multi_step tre0_ex1 gstk_M6 6 20"
-value "multi_step tre0_ex1 gstk_M6 7 20"
-value "multi_step tre0_ex1 gstk_M6 8 20"
-value "multi_step tre0_ex1 gstk_M6 9 20"
-value "multi_step tre0_ex1 gstk_M6 10 20"
-value "multi_step tre0_ex1 gstk_M6 11 20"
-value "multi_step tre0_ex1 gstk_M6 12 20"
-value "multi_step tre0_ex1 gstk_M6 13 20"
-value "multi_step tre0_ex1 gstk_M6 14 20"
-value "multi_step tre0_ex1 gstk_M6 15 20"
-value "multi_step tre0_ex1 gstk_M6 16 20"
+value "multi_step tre0_ex1 gstk_M6 1"
+value "multi_step tre0_ex1 gstk_M6 2"
+value "multi_step tre0_ex1 gstk_M6 3"
+value "multi_step tre0_ex1 gstk_M6 4"
+value "multi_step tre0_ex1 gstk_M6 5"
+value "multi_step tre0_ex1 gstk_M6 6"
+value "multi_step tre0_ex1 gstk_M6 7"
+value "multi_step tre0_ex1 gstk_M6 8"
+value "multi_step tre0_ex1 gstk_M6 9"
+value "multi_step tre0_ex1 gstk_M6 10"
+value "multi_step tre0_ex1 gstk_M6 11"
+value "multi_step tre0_ex1 gstk_M6 12"
+value "multi_step tre0_ex1 gstk_M6 13"
+value "multi_step tre0_ex1 gstk_M6 14"
+value "multi_step tre0_ex1 gstk_M6 15"
+value "multi_step tre0_ex1 gstk_M6 16"
 *)
 
-value "check_gstk_exc_stp (multi_step tre0_ex1 gstk_M6 16 20)"
+value "check_gstk_exc_stp (multi_step tre0_ex1 gstk_M6 16)"
 
 
 (*M7 --- same code as M5, but with overflow of words stack*)
 (*
-value "multi_step tre0_ex1 gstk_M7 1 20"
-value "multi_step tre0_ex1 gstk_M7 2 20"
-value "multi_step tre0_ex1 gstk_M7 3 20"
-value "multi_step tre0_ex1 gstk_M7 4 20"
-value "multi_step tre0_ex1 gstk_M7 5 20"
-value "multi_step tre0_ex1 gstk_M7 6 20"
-value "multi_step tre0_ex1 gstk_M7 7 20"
-value "multi_step tre0_ex1 gstk_M7 8 20"
-value "multi_step tre0_ex1 gstk_M7 9 20"
-value "multi_step tre0_ex1 gstk_M7 10 20"
+value "multi_step tre0_ex1 gstk_M7 1"
+value "multi_step tre0_ex1 gstk_M7 2"
+value "multi_step tre0_ex1 gstk_M7 3"
+value "multi_step tre0_ex1 gstk_M7 4"
+value "multi_step tre0_ex1 gstk_M7 5"
+value "multi_step tre0_ex1 gstk_M7 6"
+value "multi_step tre0_ex1 gstk_M7 7"
+value "multi_step tre0_ex1 gstk_M7 8"
+value "multi_step tre0_ex1 gstk_M7 9"
+value "multi_step tre0_ex1 gstk_M7 10"
 *)
 
-value "check_gstk_exc_stp (multi_step tre0_ex1 gstk_M7 10 20)"
-
+value "check_gstk_exc_stp (multi_step tre0_ex1 gstk_M7 10)"
 
 end
